\begin{proof}
    Denotemos $\Sigma = \cap_{i\in\mathcal{I}}\Sigma_i$. Como $A_n\in \Sigma$ para todo $n\in \N$, ent√£o $A_n^{c}\in \Sigma$ para todo $n$ e $\left(A_n^{c}\right)_{n=1}^\infty \subset \Sigma$. Assim $\bigcup_{n=1}^\infty \left( A_n^{c} \right)\in \Sigma$. Note bem, pelo \nameref{thm:de_morgan}, 
    \begin{equation*}
        \bigcup_{n=1}^\infty \left( A_n^{c} \right) = \left( \bigcap_{n=1}^{\infty} A_n \right)^{c} \in \Sigma.
    \end{equation*}
    Portanto $\left(\bigcup_{n=1}^\infty \left( A_n^{c} \right)\right)^{c} = \bigcap_{n=1}^{\infty} A_n \in \Sigma$.
\end{proof}